prelude/base.v
@@ -1,5 +1,36 @@
+Require Export iris.proofmode.tactics.
+From iris.program_logic Require Import wsat.
+Require Import iris.program_logic.weakestpre.
+Require Import iris.program_logic.language.
 From mathcomp Require Export ssreflect.
 From iris.prelude Require Export prelude.
 Global Set Bullet Behavior "Strict Subproofs".
 Global Open Scope general_if_scope.
 Ltac done := prelude.tactics.done.
+
+
+Section uPred_Lemmas.
+  Import uPred.
+  Context {Λ : language} {Σ : iFunctor}.
+  Implicit Types P : iProp Λ Σ.
+  Implicit Types Φ : val Λ → iProp Λ Σ.
+  Implicit Types v : val Λ.
+  Implicit Types e : expr Λ.
+
+  Definition double_exists M A ψ Q Y :=
+    @exist_elim M A (λ x, ∃ b : A, ψ x b)%I Q (λ x, @exist_elim M A _ Q (Y x)).
+  
+  Lemma wp_impl_l E e Φ Ψ :
+    ((□ ∀ v, Φ v → Ψ v) ∧ WP e @ E {{ Φ }}) ⊢ WP e @ E {{ Ψ }}.
+  Proof.
+    rewrite wp_always_l; apply wp_mono=> // v.
+  by rewrite always_elim (forall_elim v) impl_elim_l.
+  Qed.
+  Lemma wp_impl_r E e Φ Ψ :
+    (WP e @ E {{ Φ }} ∧ □ (∀ v, Φ v → Ψ v)) ⊢ WP e @ E {{ Ψ }}.
+  Proof. by rewrite comm wp_impl_l. Qed.
+  Lemma wp_mask_weaken E1 E2 e Φ :
+    E1 ⊆ E2 → WP e @ E1 {{ Φ }} ⊢ WP e @ E2 {{ Φ }}.
+  Proof. auto using wp_mask_frame_mono. Qed.
+  
+End uPred_Lemmas.
