F_mu/fundamental.v
@@ -13,7 +13,7 @@ Section typed_interp.
   Canonical Structure leibniz_val := leibnizC val.
 
   Canonical Structure leibniz_le n m := leibnizC (n ≤ m).
-
+(*
   Ltac ipropsimpl :=
     repeat
       match goal with
@@ -39,172 +39,173 @@ Section typed_interp.
   Local Hint Extern 3 (_ ⊢ (_ ∨ _))%I => rewrite -or_intro_l : itauto.
   Local Hint Extern 3 (_ ⊢ (_ ∨ _))%I => rewrite -or_intro_r : itauto.
   Local Hint Extern 2 (_ ⊢ ▷ _)%I => etransitivity; [|rewrite -later_intro] : itauto.
-  
+
   Local Ltac value_case := rewrite -wp_value/= ?to_of_val //; auto 2.
+ *)
+
+  Local Hint Extern 1 =>
+  match goal with
+    |-
+    (_
+       --------------------------------------□
+       ∃ _ : ?A, _) => let W := fresh "W" in evar (W : A); iExists W; unfold W; clear W
+  end : itauto.
+
+  Local Hint Extern 1 =>
+  match goal with
+    |-
+    (_
+       --------------------------------------□
+       ▷ _) => iNext
+  end : itauto.
+
+  Local Hint Extern 1 =>
+  match goal with
+    |-
+    (_
+       --------------------------------------□
+       (_ ∧ _)) => iSplit
+  end : itauto.
   
+  
+  Local Tactic Notation "smart_wp_bind" uconstr(ctx) ident(v) constr(Hv) uconstr(Hp) :=
+    iApply (@wp_bind _ _ _ [ctx]);
+    iApply wp_impl_l;
+    iSplit; [| iApply Hp; trivial]; cbn;
+    eapply (@always_intro _ _ _ _);
+    iIntros {v} Hv.
+              
+  Local Ltac value_case := iApply wp_value; cbn; rewrite ?to_of_val; trivial.
+
   Lemma typed_interp k Δ Γ vs e τ
         (Htyped : typed k Γ e τ)
         (Hctx : closed_ctx k Γ)
         (HC : closed_type k τ)
         (HΔ : VlistAlwaysStable Δ)
-    : length Γ = length vs →
+    : List.length Γ = List.length vs →
       Π∧ zip_with (λ τ v, interp k (` τ) (proj2_sig τ) Δ v) (closed_ctx_list _ Γ Hctx) vs ⊢
                   WP (e.[env_subst vs]) @ ⊤ {{ λ v, (@interp Σ) k τ HC Δ v }}.
   Proof.
     revert Hctx HC HΔ vs.
-    induction Htyped; intros Hctx HC HΔ vs Hlen; cbn.
+    induction Htyped; intros Hctx HC HΔ vs Hlen; iIntros "#HΓ"; cbn.
     - (* var *)
       destruct (lookup_lt_is_Some_2 vs x) as [v Hv].
       { by rewrite -Hlen; apply lookup_lt_Some with τ. }
-      rewrite /env_subst Hv /= -wp_value; eauto using to_of_val.
+      rewrite /env_subst Hv; value_case.
       edestruct (zipwith_Forall_lookup _ Hctx) as [Hτ' Hτ'eq]; eauto.
-      etransitivity.
-      apply big_and_elem_of, elem_of_list_lookup_2 with x.
+      iApply interp_closed_irrel_turnstile.
+      iApply big_and_elem_of "HΓ"; eauto.
+      apply elem_of_list_lookup_2 with x.
       rewrite lookup_zip_with; simplify_option_eq; trivial.
-      rewrite interp_closed_irrel; trivial.
     - (* unit *) value_case.
     - (* pair *)
-      smart_wp_bind (PairLCtx e2.[env_subst vs]) _ v; eauto.
-      (* weird!: and_alwaysstable is an instance but is not resolved! *)
-      smart_wp_bind (PairRCtx v) (and_persistent _ _ _ _) v'.
+      smart_wp_bind (PairLCtx e2.[env_subst vs]) v "# Hv" IHHtyped1.
+      smart_wp_bind (PairRCtx v) v' "# Hv'" IHHtyped2.
       value_case; eauto 10 with itauto.
     - (* fst *)
-      smart_wp_bind (FstCtx) v. ipropsimpl; eauto.
-      apply const_elim_l; intros H; rewrite H.
-      rewrite -wp_fst; eauto using to_of_val, and_elim_l.
-      rewrite and_elim_l; rewrite interp_closed_irrel; eauto.
+      smart_wp_bind (FstCtx) v "# Hv" IHHtyped; cbn.
+      iApply double_exists; [|trivial].
+      intros w w'; cbn; iIntros "#[% [H2 H3]]"; rewrite H; cbn.
+      iApply wp_fst; eauto using to_of_val; cbn.
+      iNext; iApply interp_closed_irrel_turnstile; trivial.
     - (* snd *)
-      smart_wp_bind SndCtx v. ipropsimpl; eauto.
-      apply const_elim_l; intros H; rewrite H.
-      rewrite -wp_snd; eauto using to_of_val, and_elim_l.
-      rewrite and_elim_r; rewrite interp_closed_irrel; eauto.
-    - (* injl *) smart_wp_bind InjLCtx v; value_case; eauto 7 with itauto.
-    - (* injr *) smart_wp_bind InjRCtx v; value_case; eauto 7 with itauto.
+      smart_wp_bind (SndCtx) v "# Hv" IHHtyped; cbn.
+      iApply double_exists; [|trivial].
+      intros w w'; cbn; iIntros "#[% [H2 H3]]"; rewrite H.
+      iApply wp_snd; eauto using to_of_val.
+      iNext; iApply interp_closed_irrel_turnstile; trivial.
+    - (* injl *)
+      smart_wp_bind (InjLCtx) v "# Hv" IHHtyped; cbn.
+      value_case; iLeft; auto with itauto.
+    - (* injr *)
+      smart_wp_bind (InjRCtx) v "# Hv" IHHtyped; cbn.
+      value_case; iRight; auto with itauto.
     - (* case *)
-      smart_wp_bind (CaseCtx _ _) _ v. cbn.
-      rewrite (later_intro (Π∧ zip_with
-           (λ (τ : {τ : type | closed_type k τ}) (v0 : leibniz_val),
-            ((interp k (` τ) (proj2_sig τ)) Δ) v0) (closed_ctx_list k Γ Hctx) vs));
-        rewrite or_elim; [apply impl_elim_l| |].
-      + rewrite exist_elim; eauto; intros v'.
-        apply const_elim_l; intros H; rewrite H.
-        rewrite -impl_intro_r //; rewrite -later_and later_mono; eauto.
-        rewrite -wp_case_inl; eauto using to_of_val.
-        asimpl.
-        specialize (IHHtyped2 Δ (typed_closed_ctx _ _ _ _ Htyped2) HC HΔ (v'::vs)).
-        erewrite <- ?typed_subst_head_simpl in * by (cbn; eauto).
-        rewrite -IHHtyped2; cbn; auto.
-        rewrite interp_closed_irrel type_context_closed_irrel /closed_ctx_list.
-        apply later_mono, and_intro; eauto 3 with itauto.
-      + rewrite exist_elim; eauto; intros v'.
-        apply const_elim_l; intros H; rewrite H.
-        rewrite -impl_intro_r //; rewrite -later_and later_mono; eauto.
-        rewrite -wp_case_inr; eauto using to_of_val.
-        asimpl.
-        specialize (IHHtyped3 Δ (typed_closed_ctx _ _ _ _ Htyped3) HC HΔ (v'::vs)).
-        erewrite <- ?typed_subst_head_simpl in * by (cbn; eauto).
-        rewrite -IHHtyped3; cbn; auto.
-        rewrite interp_closed_irrel type_context_closed_irrel /closed_ctx_list.
-        apply later_mono, and_intro; eauto 3 with itauto.    
+      smart_wp_bind (CaseCtx _ _) v "#Hv" IHHtyped1; cbn.
+      iDestruct "Hv" as "[Hv|Hv]"; eauto; iRevert "HΓ";
+        iApply exist_elim; eauto; cbn;
+          iIntros {w} "#[% Hw2] #HΓ"; rewrite H; cbn;
+            [iApply wp_case_inl|iApply wp_case_inr];
+            auto 1 using to_of_val;
+            asimpl;
+            [specialize (IHHtyped2 Δ (typed_closed_ctx _ _ _ _ Htyped2) HC HΔ (w::vs)) |
+             specialize (IHHtyped3 Δ (typed_closed_ctx _ _ _ _ Htyped3) HC HΔ (w::vs))];
+              erewrite <- ?typed_subst_head_simpl in * by (cbn; eauto); iNext;
+                [iApply IHHtyped2 | iApply IHHtyped3]; cbn; auto;
+                  (iSplit; [iApply interp_closed_irrel_turnstile|
+                            iApply type_context_closed_irrel_turnstile]; trivial).
     - (* lam *)
-      value_case; apply (always_intro _ _), forall_intro=> v /=; apply impl_intro_l.
-      rewrite -wp_lam ?to_of_val //=.
-      asimpl. erewrite typed_subst_head_simpl; [|eauto|cbn]; eauto.
-      rewrite (later_intro (Π∧ _)) -later_and; apply later_mono.
-      rewrite interp_closed_irrel type_context_closed_irrel /closed_ctx_list.
-      rewrite -(IHHtyped Δ (typed_closed_ctx _ _ _ _ Htyped) (closed_type_arrow_2 HC) HΔ (v :: vs));
-        simpl; auto with f_equal.
+      value_case; apply (always_intro _ _); iIntros {w} "#Hw".
+      iApply wp_lam; auto 1 using to_of_val.
+      asimpl; erewrite typed_subst_head_simpl; [|eauto|cbn]; eauto.
+      iNext; iApply (IHHtyped Δ (typed_closed_ctx _ _ _ _ Htyped) (closed_type_arrow_2 HC)
+                              HΔ (w :: vs)); cbn; auto.
+      (iSplit; [iApply interp_closed_irrel_turnstile|
+                iApply type_context_closed_irrel_turnstile]; trivial).
     - (* app *)
-      smart_wp_bind (AppLCtx (e2.[env_subst vs])) _ v.
-      rewrite -(@wp_bind _ _ _ [AppRCtx v]) /=.
-      rewrite -wp_impl_l /=; apply and_intro.
-      2: etransitivity; [|apply IHHtyped2]; eauto using and_elim_r.
-      rewrite and_elim_l. apply always_mono.
-      apply forall_intro =>v'.
-      rewrite forall_elim.
-      apply impl_intro_l.
-      rewrite -(later_intro).
-      etransitivity; [apply impl_elim_r|].
-      apply wp_mono => w.
-      rewrite interp_closed_irrel; trivial.
+      smart_wp_bind (AppLCtx (e2.[env_subst vs])) v "#Hv" IHHtyped1.
+      smart_wp_bind (AppRCtx v) w "#Hw" IHHtyped2.
+      iApply wp_mono; [|iApply "Hv"; auto with itauto].
+      intros; apply interp_closed_irrel_turnstile.
     - (* TLam *)
-      value_case; rewrite -exist_intro; apply and_intro; auto.
-      apply forall_intro =>τi;
-        apply (always_intro _ _).
-      rewrite map_length in IHHtyped.
-      destruct τi as [τi τiAS].
-      specialize (IHHtyped
-                    (Vlist_cons τi Δ)
-                    (closed_ctx_map
-                       _ _ _ _
-                       Hctx (λ τ, closed_type_S_ren2 τ 1 0 _))
-                    (closed_type_forall HC)
-                    (alwyas_stable_Vlist_cons _ _ _ τiAS)
-                    _
-                    Hlen
-                 ).
-      rewrite -wp_impl_l -later_intro. apply and_intro;
-        [ apply (always_intro _ _), forall_intro=> v /=; apply impl_intro_l|].
-      2: etransitivity; [|apply IHHtyped].
-      + rewrite and_elim_l; trivial.
-      + rewrite zip_with_closed_ctx_list_subst; trivial.
+      value_case; iApply exist_intro; iSplit; trivial.
+      iIntros {τi}; destruct τi as [τi τiPr].
+      iPoseProof always_intro "HΓ" as "HP"; try typeclasses eauto; try iExact "HP".
+      iIntros "#HΓ"; iNext.
+      iApply IHHtyped; [rewrite map_length|]; trivial.
+      iRevert "HΓ".
+      rewrite zip_with_closed_ctx_list_subst.
+      iIntros "#HΓ"; trivial.
     - (* TApp *)
-      smart_wp_bind TAppCtx _ v; cbn.
-      rewrite and_elim_l.
-      rewrite exist_elim; eauto => e'.
-      apply const_elim_l; intros H'; rewrite H'.
-      rewrite (forall_elim ((interp k τ' H Δ) ↾ _)).
-      rewrite always_elim.
-      rewrite -wp_TLam; apply later_mono.
-      apply wp_mono=> w.
-      rewrite interp_subst; trivial.
+      smart_wp_bind TAppCtx v "#Hv" IHHtyped; cbn.
+      iApply exist_elim; [|iExact "Hv"]; cbn.
+      iIntros {e'} "[% #He']"; rewrite H0.
+      iApply wp_TLam.
+      iSpecialize "He'" {((interp k τ' H Δ) ↾ _)}; cbn.
+      iApply always_elim. iApply always_mono; [|trivial].
+      iIntros "He'"; iNext.
+      iApply wp_mono; [|trivial].
+      intros w; rewrite interp_subst; trivial.
     - (* Fold *)
-      value_case. unfold interp_rec.
-      rewrite fixpoint_unfold.
-      cbn.
-      rewrite -exist_intro.
-      apply (always_intro _ _).
-      apply and_intro; auto.
       rewrite map_length in IHHtyped.
-      specialize (IHHtyped
-                    (Vlist_cons (interp k (TRec τ) HC Δ) Δ)
-                    (closed_ctx_map
-                       _ _ _ _
-                       Hctx (λ τ, closed_type_S_ren2 τ 1 0 _))
-                    (closed_type_rec HC)
-                    (alwyas_stable_Vlist_cons _ _ _ _)
-                   _
-                    Hlen
-                 ).      
-      rewrite -wp_impl_l -later_intro. apply and_intro;
-        [ apply (always_intro _ _), forall_intro=> v /=; apply impl_intro_l|].
-      2: etransitivity; [|apply IHHtyped].
-      + rewrite and_elim_l; trivial.
-      + rewrite zip_with_closed_ctx_list_subst; trivial.
+      iApply (@wp_bind _ _ _ [FoldCtx]);
+        iApply wp_impl_l;
+        iSplit; [eapply (@always_intro _ _ _ _)|
+                 iApply (IHHtyped _ _ (closed_type_rec HC)); trivial]; cbn.
+      + iIntros {v} "#Hv".
+        value_case. rewrite /interp_rec fixpoint_unfold. unfold interp_rec_pre at 1; cbn.
+        eapply (@always_intro _ _ _ _).
+        iApply exist_intro; iSplit; trivial.
+        iNext.
+        change (fixpoint (interp_rec_pre
+                            (Vlist_cons_apply Δ (interp (S k) τ (closed_type_rec HC)))))
+        with ((interp k (TRec τ) HC) Δ); trivial.
+      + iRevert "HΓ"; rewrite zip_with_closed_ctx_list_subst; iIntros "#HΓ"; trivial.
     - (* Unfold *)
-      smart_wp_bind UnfoldCtx _ v; cbn.
-      rewrite and_elim_l.
-      unfold interp_rec. rewrite fixpoint_unfold /interp_rec_pre; cbn.
-      replace (fixpoint
-                 (λ rec_apr : leibniz_val -n> iProp lang Σ,
-                              CofeMor
-                                (λ w : leibniz_val,
-                                       □ (∃ e1 : expr,
-                                             w = FoldV e1
-                                             ∧ ▷ WP e1 @ ⊤ {{ λ v1 : val,
-                                                        ((interp (S k) τ (closed_type_rec ?HC4))
-                                                           (Vlist_cons rec_apr Δ)) v1 }}))%I))
-      with
-      (interp k (TRec τ) (typed_closed_type _ _ _ _ Htyped) Δ) by (cbn; unfold interp_rec; trivial).
-      rewrite always_elim.
-      rewrite exist_elim; eauto => e'.
-      apply const_elim_l; intros H'; rewrite H'.
-      rewrite -wp_Fold.
-      apply later_mono, wp_mono => w.
-      rewrite -interp_subst; eauto.
+      iApply (@wp_bind _ _ _ [UnfoldCtx]);
+        iApply wp_impl_l;
+        iSplit; [eapply (@always_intro _ _ _ _)|
+                 iApply (IHHtyped _ _ (typed_closed_type _ _ _ _ Htyped)); trivial]; cbn.
+      iIntros {v}.
+      rewrite /interp_rec fixpoint_unfold. unfold interp_rec_pre at 1; cbn.
+      iIntros "#Hv".
+      iApply exist_elim; [|iAssumption].
+      iIntros {w}; cbn.
+      change (fixpoint (interp_rec_pre
+                          (Vlist_cons_apply
+                             Δ
+                             (interp
+                                (S k) τ
+                                (closed_type_rec
+                                   (typed_closed_type k Γ e (TRec τ) Htyped))))))
+      with ((interp k (TRec τ) (typed_closed_type k Γ e (TRec τ) Htyped)) Δ); trivial.
+      iIntros "[% #Hw]"; rewrite H.
+      iApply wp_Fold; cbn; auto using to_of_val.
+      iRevert "Hw". rewrite -interp_subst. iIntros "#Hw". trivial.
       (* unshelving *)
       Unshelve.
-      all: solve [eauto 2 using typed_closed_type | try typeclasses eauto].
+      all: cbn; solve [eauto 2 using closed_ctx_map_S_back,
+                       typed_closed_type | try typeclasses eauto].
   Qed.
   
 End typed_interp.
