F_mu_ref/fundamental.v
@@ -18,6 +18,7 @@ Section typed_interp.
   Implicit Types P Q R : iPropG lang Σ.
   Notation "# v" := (of_val v) (at level 20).
 
+  (*
   Local Ltac ipropsimpl :=
     repeat
       match goal with
@@ -45,6 +46,44 @@ Section typed_interp.
   Local Hint Extern 2 (_ ⊢ ▷ _)%I => etransitivity; [|rewrite -later_intro] : itauto.
   
   Local Ltac value_case := rewrite -wp_value/= ?to_of_val //; auto 2.
+*)
+
+  Local Hint Extern 1 =>
+  match goal with
+    |-
+    (_
+       --------------------------------------□
+       ∃ _ : ?A, _) => let W := fresh "W" in evar (W : A); iExists W; unfold W; clear W
+  end : itauto.
+
+  Local Hint Extern 1 =>
+  match goal with
+    |-
+    (_
+       --------------------------------------□
+       ▷ _) => iNext
+  end : itauto.
+
+  Local Hint Extern 1 =>
+  match goal with
+    |-
+    (_
+       --------------------------------------□
+       (_ ∧ _)) => iSplit
+  end : itauto.
+  
+  
+  Local Tactic Notation "smart_wp_bind" uconstr(ctx) ident(v) constr(Hv) uconstr(Hp) :=
+    iApply (@wp_bind _ _ _ [ctx]);
+    iApply wp_impl_l;
+    iSplit; [| iApply Hp; trivial];
+    [apply (always_intro _ _); iIntros {v} Hv|iSplit; trivial]; cbn.
+              
+  Local Ltac value_case := iApply wp_value; cbn; rewrite ?to_of_val; trivial.
+
+  Lemma later_exist_turnstile (M : cmraT) (A : Type) :
+    Inhabited A → ∀ Φ : A → uPred M, (▷ (∃ a : A, Φ a))%I ⊢ (∃ a : A, ▷ Φ a)%I.
+  Proof. intros H Φ. rewrite later_exist; trivial. Qed.
 
   Lemma typed_interp N k Δ Γ vs e τ
         (HNLdisj : ∀ l : loc, N ⊥ L .@ l)
@@ -52,255 +91,192 @@ Section typed_interp.
         (Hctx : closed_ctx k Γ)
         (HC : closed_type k τ)
         (HΔ : VlistAlwaysStable Δ)
-    : length Γ = length vs →
+    : List.length Γ = List.length vs →
       (heap_ctx N ∧ Π∧ zip_with (λ τ v, (@interp Σ i L) k (` τ) (proj2_sig τ) Δ v) (closed_ctx_list _ Γ Hctx) vs)%I ⊢
                   WP (e.[env_subst vs]) @ ⊤ {{ λ v, (@interp Σ i L) k τ HC Δ v }}.
   Proof.
     revert Hctx HC HΔ vs.
-    induction Htyped; intros Hctx HC HΔ vs Hlen; cbn.
+    induction Htyped; intros Hctx HC HΔ vs Hlen; iIntros "#[Hheap HΓ]"; cbn.
     - (* var *)
       destruct (lookup_lt_is_Some_2 vs x) as [v Hv].
       { by rewrite -Hlen; apply lookup_lt_Some with τ. }
-      rewrite /env_subst Hv /= -wp_value; eauto using to_of_val.
+      rewrite /env_subst Hv; value_case.
       edestruct (zipwith_Forall_lookup _ Hctx) as [Hτ' Hτ'eq]; eauto.
-      rewrite and_elim_r.
-      etransitivity.
-      apply big_and_elem_of, elem_of_list_lookup_2 with x.
+      iApply interp_closed_irrel_turnstile.
+      iApply big_and_elem_of "HΓ"; eauto.
+      apply elem_of_list_lookup_2 with x.
       rewrite lookup_zip_with; simplify_option_eq; trivial.
-      rewrite interp_closed_irrel; trivial.
     - (* unit *) value_case.
     - (* pair *)
-      smart_wp_bind (PairLCtx e2.[env_subst vs]) _ v; eauto.
-      (* weird!: and_alwaysstable is an instance but is not resolved! *)
-      smart_wp_bind (PairRCtx v) (and_persistent _ _ _ _) v'.
+      smart_wp_bind (PairLCtx e2.[env_subst vs]) v "#Hv" IHHtyped1.
+      smart_wp_bind (PairRCtx v) v' "# Hv'" IHHtyped2.
       value_case; eauto 10 with itauto.
     - (* fst *)
-      smart_wp_bind (FstCtx) v. ipropsimpl; eauto.
-      apply const_elim_l; intros H; rewrite H.
-      rewrite -wp_fst; eauto using to_of_val, and_elim_l.
-      rewrite and_elim_l; rewrite interp_closed_irrel; eauto.
+      smart_wp_bind (FstCtx) v "# Hv" IHHtyped; cbn.
+      iApply double_exists; [|trivial].
+      intros w w'; cbn; iIntros "#[% [H2 H3]]"; rewrite H; cbn.
+      iApply wp_fst; eauto using to_of_val; cbn.
+      iNext; iApply interp_closed_irrel_turnstile; trivial.
     - (* snd *)
-      smart_wp_bind SndCtx v. ipropsimpl; eauto.
-      apply const_elim_l; intros H; rewrite H.
-      rewrite -wp_snd; eauto using to_of_val, and_elim_l.
-      rewrite and_elim_r; rewrite interp_closed_irrel; eauto.
-    - (* injl *) smart_wp_bind InjLCtx v; value_case; eauto 7 with itauto.
-    - (* injr *) smart_wp_bind InjRCtx v; value_case; eauto 7 with itauto.
+      smart_wp_bind (SndCtx) v "# Hv" IHHtyped; cbn.
+      iApply double_exists; [|trivial].
+      intros w w'; cbn; iIntros "#[% [H2 H3]]"; rewrite H; cbn.
+      iApply wp_snd; eauto using to_of_val; cbn.
+      iNext; iApply interp_closed_irrel_turnstile; trivial.
+    - (* injl *)
+      smart_wp_bind (InjLCtx) v "# Hv" IHHtyped; cbn.
+      value_case; iLeft; auto with itauto.
+    - (* injr *)
+      smart_wp_bind (InjRCtx) v "# Hv" IHHtyped; cbn.
+      value_case; iRight; auto with itauto.
     - (* case *)
-      smart_wp_bind (CaseCtx _ _) _ v. cbn.
-      rewrite (later_intro (heap_ctx N ∧ Π∧ zip_with
-           (λ (τ : {τ : type | closed_type k τ}) (v0 : leibniz_val),
-            ((interp k (` τ) (proj2_sig τ)) Δ) v0) (closed_ctx_list k Γ Hctx) vs));
-        rewrite or_elim; [apply impl_elim_l| |].
-      + rewrite exist_elim; eauto; intros v'.
-        apply const_elim_l; intros H; rewrite H.
-        rewrite -impl_intro_r //; rewrite -later_and later_mono; eauto.
-        rewrite -wp_case_inl; eauto using to_of_val.
-        asimpl.
-        specialize (IHHtyped2 Δ (typed_closed_ctx _ _ _ _ Htyped2) HC HΔ (v'::vs)).
-        erewrite <- ?typed_subst_head_simpl in * by (cbn; eauto).
-        rewrite -IHHtyped2; cbn; auto.
-        rewrite interp_closed_irrel type_context_closed_irrel /closed_ctx_list.
-        apply later_mono; repeat apply and_intro; eauto 3 with itauto.
-      + rewrite exist_elim; eauto; intros v'.
-        apply const_elim_l; intros H; rewrite H.
-        rewrite -impl_intro_r //; rewrite -later_and later_mono; eauto.
-        rewrite -wp_case_inr; eauto using to_of_val.
-        asimpl.
-        specialize (IHHtyped3 Δ (typed_closed_ctx _ _ _ _ Htyped3) HC HΔ (v'::vs)).
-        erewrite <- ?typed_subst_head_simpl in * by (cbn; eauto).
-        rewrite -IHHtyped3; cbn; auto.
-        rewrite interp_closed_irrel type_context_closed_irrel /closed_ctx_list.
-        apply later_mono; repeat apply and_intro; eauto 3 with itauto.
+      smart_wp_bind (CaseCtx _ _) v "#Hv" IHHtyped1; cbn.
+      iDestruct "Hv" as "[Hv|Hv]"; eauto; iRevert "HΓ"; iRevert "Hheap";
+        iApply exist_elim; eauto; cbn;
+          iIntros {w} "#[% Hw2] #HΓ #Hheap"; rewrite H; cbn;
+            [iApply wp_case_inl|iApply wp_case_inr];
+            auto 1 using to_of_val;
+            asimpl;
+            [specialize (IHHtyped2 Δ (typed_closed_ctx _ _ _ _ Htyped2) HC HΔ (w::vs)) |
+             specialize (IHHtyped3 Δ (typed_closed_ctx _ _ _ _ Htyped3) HC HΔ (w::vs))];
+              erewrite <- ?typed_subst_head_simpl in * by (cbn; eauto); iNext;
+                [iApply IHHtyped2 | iApply IHHtyped3]; cbn; auto;
+                  (iSplit; [trivial|iSplit]; [iApply interp_closed_irrel_turnstile|
+                            iApply type_context_closed_irrel_turnstile]; trivial).
     - (* lam *)
-      value_case; apply (always_intro _ _), forall_intro=> v /=; apply impl_intro_l.
-      rewrite -wp_lam ?to_of_val //=.
-      asimpl. erewrite typed_subst_head_simpl; [|eauto|cbn]; eauto.
-      rewrite (later_intro (heap_ctx N ∧ Π∧ _)) -later_and; apply later_mono.
-      rewrite interp_closed_irrel type_context_closed_irrel /closed_ctx_list.
-      rewrite -(IHHtyped Δ (typed_closed_ctx _ _ _ _ Htyped) (closed_type_arrow_2 HC) HΔ (v :: vs)); cbn; auto 2 with f_equal.
-      repeat apply and_intro; eauto 3 with itauto.
+      value_case; apply (always_intro _ _); iIntros {w} "#Hw".
+      iApply wp_lam; auto 1 using to_of_val.
+      asimpl; erewrite typed_subst_head_simpl; [|eauto|cbn]; eauto.
+      iNext; iApply (IHHtyped Δ (typed_closed_ctx _ _ _ _ Htyped) (closed_type_arrow_2 HC)
+                              HΔ (w :: vs)); cbn; auto.
+      (iSplit; [trivial|iSplit]; [iApply interp_closed_irrel_turnstile|
+                iApply type_context_closed_irrel_turnstile]; trivial).
     - (* app *)
-      smart_wp_bind (AppLCtx (e2.[env_subst vs])) _ v.
-      rewrite -(@wp_bind _ _ _ [AppRCtx v]) /=.
-      rewrite -wp_impl_l /=; apply and_intro.
-      2: etransitivity; [|apply IHHtyped2]; eauto using and_elim_r.
-      rewrite and_elim_l. apply always_mono.
-      apply forall_intro =>v'.
-      rewrite forall_elim.
-      apply impl_intro_l.
-      rewrite -(later_intro).
-      etransitivity; [apply impl_elim_r|].
-      apply wp_mono => w.
-      rewrite interp_closed_irrel; trivial.
+      smart_wp_bind (AppLCtx (e2.[env_subst vs])) v "#Hv" IHHtyped1.
+      smart_wp_bind (AppRCtx v) w "#Hw" IHHtyped2.
+      iApply wp_mono; [|iApply "Hv"; auto with itauto].
+      intros; apply interp_closed_irrel_turnstile.
     - (* TLam *)
-      value_case; rewrite -exist_intro; apply and_intro; auto.
-      apply forall_intro =>τi;
-        apply (always_intro _ _).
-      rewrite map_length in IHHtyped.
-      destruct τi as [τi τiAS].
-      specialize (IHHtyped
-                    (Vlist_cons τi Δ)
-                    (closed_ctx_map
-                       _ _ _ _
-                       Hctx (λ τ, closed_type_S_ren2 τ 1 0 _))
-                    (closed_type_forall HC)
-                    (alwyas_stable_Vlist_cons _ _ _ τiAS)
-                    _
-                    Hlen
-                 ).
-      rewrite -wp_impl_l -later_intro. apply and_intro;
-        [ apply (always_intro _ _), forall_intro=> v /=; apply impl_intro_l|].
-      2: etransitivity; [|apply IHHtyped].
-      + rewrite and_elim_l; trivial.
-      + rewrite zip_with_closed_ctx_list_subst; trivial.
+      value_case; iApply exist_intro; iSplit; trivial.
+      iIntros {τi}; destruct τi as [τi τiPr].
+      iRevert "Hheap".
+      iPoseProof always_intro "HΓ" as "HP"; try typeclasses eauto;
+        try (iApply always_impl; iExact "HP").
+      iIntros "#HΓ #Hheap"; iNext.
+      iApply IHHtyped; [rewrite map_length|]; trivial.
+      iSplit; trivial.
+      iRevert "HΓ". rewrite zip_with_closed_ctx_list_subst. iIntros "#HΓ"; trivial.
     - (* TApp *)
-      smart_wp_bind TAppCtx _ v; cbn.
-      rewrite and_elim_l.
-      rewrite exist_elim; eauto => e'.
-      apply const_elim_l; intros H'; rewrite H'.
-      rewrite (forall_elim ((interp k τ' H Δ) ↾ _)).
-      rewrite always_elim.
-      rewrite -wp_TLam; apply later_mono.
-      apply wp_mono=> w.
-      eapply entails_proper.
-      + apply interp_subst.
-      + eauto.
-      + eauto.
+      smart_wp_bind TAppCtx v "#Hv" IHHtyped; cbn.
+      iApply exist_elim; [|iExact "Hv"]; cbn.
+      iIntros {e'} "[% #He']"; rewrite H0.
+      iApply wp_TLam.
+      iSpecialize "He'" {((interp k τ' H Δ) ↾ _)}; cbn.
+      iApply always_elim. iApply always_mono; [|trivial].
+      iIntros "He'"; iNext.
+      iApply wp_mono; [|trivial].
+      intros w; cbn; rewrite -interp_subst; trivial.
     - (* Fold *)
-      value_case. unfold interp_rec.
-      rewrite fixpoint_unfold.
-      cbn.
-      rewrite -exist_intro.
-      apply (always_intro _ _).
-      apply and_intro; auto.
       rewrite map_length in IHHtyped.
-      specialize (IHHtyped
-                    (Vlist_cons (@interp Σ i L k (TRec τ) HC Δ) Δ)
-                    (closed_ctx_map
-                       _ _ _ _
-                       Hctx (λ τ, closed_type_S_ren2 τ 1 0 _))
-                    (closed_type_rec HC)
-                    (alwyas_stable_Vlist_cons _ _ _ _)
-                   _
-                    Hlen
-                 ).      
-      rewrite -wp_impl_l -later_intro. apply and_intro;
-        [ apply (always_intro _ _), forall_intro=> v /=; apply impl_intro_l|].
-      2: etransitivity; [|apply IHHtyped].
-      + rewrite and_elim_l; trivial.
-      + rewrite zip_with_closed_ctx_list_subst; trivial.
+      iApply (@wp_bind _ _ _ [FoldCtx]);
+        iApply wp_impl_l;
+        iSplit; [eapply (@always_intro _ _ _ _)|
+                 iApply (IHHtyped _ _ (closed_type_rec HC)); trivial]; cbn.
+      + iIntros {v} "#Hv".
+        value_case. rewrite /interp_rec fixpoint_unfold. unfold interp_rec_pre at 1; cbn.
+        eapply (@always_intro _ _ _ _).
+        iApply exist_intro; iSplit; trivial.
+        iNext.
+        change (fixpoint (interp_rec_pre
+                            (Vlist_cons_apply Δ (interp (S k) τ (closed_type_rec HC)))))
+        with ((@interp _ _ L k (TRec τ) HC) Δ); trivial.
+      + iRevert "HΓ"; rewrite zip_with_closed_ctx_list_subst; iIntros "#HΓ";
+          iSplit; trivial.
     - (* Unfold *)
-      smart_wp_bind UnfoldCtx _ v; cbn.
-      rewrite and_elim_l.
-      unfold interp_rec. rewrite fixpoint_unfold /interp_rec_pre; cbn.
-      replace (fixpoint
-                 (λ rec_apr : leibniz_val -n> iPropG lang Σ,
-                              CofeMor
-                                (λ w : leibniz_val,
-                                       □ (∃ e1 : expr,
-                                             w = FoldV e1
-                                             ∧ ▷ WP e1 @ ⊤ {{ λ v1 : val,
-                                                        ((interp (S k) τ (closed_type_rec ?HC4))
-                                                           (Vlist_cons rec_apr Δ)) v1 }}))%I))
-      with
-      (@interp Σ i L k (TRec τ) (typed_closed_type _ _ _ _ Htyped) Δ) by (cbn; unfold interp_rec; trivial).
-      rewrite always_elim.
-      rewrite exist_elim; eauto => e'.
-      apply const_elim_l; intros H'; rewrite H'.
-      rewrite -wp_Fold.
-      apply later_mono, wp_mono => w.
-      rewrite -interp_subst; eauto.
+      iApply (@wp_bind _ _ _ [UnfoldCtx]);
+        iApply wp_impl_l;
+        iSplit; [eapply (@always_intro _ _ _ _)|
+                 iApply (IHHtyped _ _ (typed_closed_type _ _ _ _ Htyped)); trivial];
+        [|iSplit; trivial]; cbn.
+      iIntros {v}.
+      rewrite /interp_rec fixpoint_unfold. unfold interp_rec_pre at 1; cbn.
+      iIntros "#Hv".
+      iApply exist_elim; [|iAssumption].
+      iIntros {w}; cbn.
+      change (fixpoint (interp_rec_pre
+                          (Vlist_cons_apply
+                             Δ
+                             (interp
+                                (S k) τ
+                                (closed_type_rec
+                                   (typed_closed_type k Γ e (TRec τ) Htyped))))))
+      with ((@interp _ _ L k (TRec τ) (typed_closed_type k Γ e (TRec τ) Htyped)) Δ);
+        trivial.
+      iIntros "[% #Hw]"; rewrite H.
+      iApply wp_Fold; cbn; auto using to_of_val.
+      iRevert "Hw". rewrite -interp_subst. iIntros "#Hw". trivial.
     - (* Alloc *)
-      smart_wp_bind AllocCtx _ v; cbn.
-      rewrite -wp_atomic; cbn; eauto using to_of_val.
-      rewrite -wp_alloc.
-      apply pvs_intro.
-      all : eauto 3 using to_of_val with itauto.
-      rewrite -later_intro.
-      apply forall_intro => l.
-      apply wand_intro_l.
-      rewrite -exist_intro.
-      rewrite -pvs_always_l.
-      apply and_intro; auto.
-      rewrite -inv_alloc; auto.
-      rewrite -later_intro /interp_ref_pred.
-      rewrite -exist_intro.
-      apply sep_mono; eauto.
-      auto with itauto.
+      smart_wp_bind AllocCtx v "#Hv" IHHtyped; cbn. iClear "HΓ".
+      iApply wp_atomic; cbn; trivial; [rewrite to_of_val; auto|].
+      iApply pvs_intro.
+      iApply wp_alloc; [| | | |iSplit;[iExact "Hheap"|iExact "Hv"]];
+        [|iIntros "#[Hheap Hv]"| |]; auto using to_of_val.
+      iIntros "#[Hheap Hv]". iNext.
+      iIntros {l} "Hl".
+      iApply exist_intro.
+      iApply and_intro; [| trivial |]; auto.
+      iApply inv_alloc; trivial. iNext.
+      iApply exist_intro.
+      iSplit; trivial.
     - (* Load *)
-      smart_wp_bind LoadCtx _ v; cbn.
-      rewrite and_exist_r. apply exist_elim => l.
-      rewrite -and_assoc.
-      apply const_elim_l; intros Heq; rewrite Heq.
-      rewrite -wp_atomic; cbn; eauto using to_of_val.
-      rewrite -wp_inv; try match goal with |- _ ⊆ _ => trivial end.
-      rewrite -pvs_intro; eauto.
-      cbn; eauto using to_of_val.
-      apply and_elim_l.
-      rewrite and_elim_r and_elim_l.
-      apply wand_intro_l.
-      unfold interp_ref_pred at 1.
-      apply wand_elim_l'.
-      etrans; [rewrite later_exist|]; eauto.
-      rewrite exist_elim; eauto => w.
-      apply wand_intro_r.
-      rewrite -(wp_load _ _ _ 1); try match goal with |- _ ⊆ _ => trivial end; eauto.
-      rewrite sep_elim_r; auto with itauto.
+      smart_wp_bind LoadCtx v "#Hv" IHHtyped; cbn. iClear "HΓ".
+      iRevert "Hheap". iApply exist_elim; [|iExact "Hv"].
+      iIntros {l} "[% #Hv] #Hheap"; rewrite H.
+      iApply wp_atomic; cbn; eauto using to_of_val.
+      iApply wp_inv; [auto using to_of_val| trivial
+                      | apply and_elim_r | apply and_elim_l | ].
+      iApply pvs_intro. iSplit; trivial.
+      iIntros "Hl".
+      iPoseProof later_exist_turnstile "Hl" as "Hl'"; [typeclasses eauto|].
+      iRevert "Hheap".
+      iApply exist_elim; [|iExact "Hl'"].
+      iIntros {w} "[Hl1 #Hl2] #Hheap".
+      iApply (wp_load _ _ _ 1);
+        [apply and_elim_r| trivial | apply and_elim_l | iSplit; trivial].
       specialize (HNLdisj l); set_solver_ndisj.
-      rewrite sep_elim_l.
-      unfold interp_ref_pred.
-      rewrite -later_sep.
-      apply later_mono.
-      apply sep_mono; eauto.
-      apply wand_intro_l.
-      rewrite -later_intro.
-      rewrite -exist_intro.
-      rewrite (always_sep_dup (((interp k τ (closed_type_ref _)) Δ) w)).
-      rewrite sep_assoc.
-      apply sep_mono; eauto.
-      rewrite -pvs_intro.
-      rewrite interp_closed_irrel; trivial.
+      iNext.
+      iSplitL; trivial.
+      iIntros "Hl".
+      iSplitL.
+      + iNext. iApply exist_intro; iSplitL; trivial.
+      + iApply pvs_intro; iApply interp_closed_irrel_turnstile; trivial.
     - (* Store *)
-      smart_wp_bind (StoreLCtx _) _ v; cbn.
-      smart_wp_bind (StoreRCtx _) _ v'; cbn.
-      rewrite and_comm ?and_assoc.
-      rewrite !and_exist_r. apply exist_elim => l.
-      rewrite -!and_assoc.
-      apply const_elim_l; intros Heq; rewrite Heq.
-      rewrite -wp_atomic; cbn; eauto using to_of_val.
-      rewrite -wp_inv; try match goal with |- _ ⊆ _ => trivial end.
-      rewrite -pvs_intro; eauto.
-      cbn; eauto using to_of_val.
-      apply and_elim_l.
-      rewrite and_elim_r and_comm -and_assoc and_elim_r.
-      apply wand_intro_l.
-      unfold interp_ref_pred at 1.
-      apply wand_elim_l'.
-      etrans; [rewrite later_exist|]; eauto.
-      rewrite exist_elim; eauto => w.
-      apply wand_intro_r.
-      rewrite -wp_store; try match goal with |- _ ⊆ _ => trivial end; eauto using to_of_val.
-      rewrite sep_elim_r; auto with itauto.
+      smart_wp_bind (StoreLCtx _) v "#Hv" IHHtyped1; cbn.
+      smart_wp_bind (StoreRCtx _) w "#Hw" IHHtyped2; cbn. iClear "HΓ".
+      iRevert "Hheap Hw". iApply exist_elim; [|iExact "Hv"].
+      iIntros {l} "#[% Hl] #Hheap #Hw"; rewrite H.
+      iApply wp_atomic; cbn; [trivial| rewrite ?to_of_val; auto |].
+      iApply wp_inv; [cbn; rewrite ?to_of_val; auto| trivial
+                      | apply and_elim_r | apply and_elim_l | ].
+      iApply pvs_intro. iSplit; trivial.
+      iClear "Hl". iIntros "Hl".
+      iPoseProof later_exist_turnstile "Hl" as "Hl'"; [typeclasses eauto|].
+      iRevert "Hheap Hw".
+      iApply exist_elim; [|iExact "Hl'"].
+      iIntros {u} "[Hl1 #Hl2] #Hheap #Hw".
+      iApply wp_store;
+        [rewrite to_of_val; trivial | apply and_elim_r
+         | | apply and_elim_l | iSplit; trivial]. 
       specialize (HNLdisj l); set_solver_ndisj.
-      rewrite and_elim_l.
-      unfold interp_ref_pred.
-      rewrite (later_intro (((interp k τ _) Δ) v')).
-      rewrite -!later_sep.
-      apply later_mono.
-      rewrite -wand_intro_l.
-      apply sep_mono. apply sep_elim_l.
-      trivial.
-      rewrite -later_intro.
-      rewrite -exist_intro.
-      rewrite (always_sep_dup (((interp k τ _) Δ) _)).
-      rewrite sep_assoc.
-      apply sep_mono; eauto.
-      rewrite interp_closed_irrel; trivial.
-      rewrite -pvs_intro; auto.
+      iSplitL; trivial.
+      iNext. iIntros "Hl".
+      iSplitL; [|iApply pvs_intro; trivial].
+      iNext. iApply exist_intro; iSplitL; trivial.
+      iApply interp_closed_irrel_turnstile; trivial.
       (* unshelving *)
       Unshelve.
-      all: solve [eauto 2 using typed_closed_type | try typeclasses eauto].
+      all: cbn; solve [eauto 2 using closed_ctx_map_S_back,
+                       typed_closed_type | try typeclasses eauto].
   Qed.
   
 End typed_interp.
